Experiment with ArithmeticExpr

hello.lean
@@ -1,32 +1,32 @@
 lemma ℕ_addition_commutative
 (n m : ℕ) : 
-n + m = m + n :=
+    n + m = m + n :=
 by cc
 -- TODO why simp failed?
 
 lemma function_currying_right_associative
 (σ τ ν : Type) : 
-( σ → τ → ν ) = ( σ → (τ → ν) ) :=
+    ( σ → τ → ν ) = ( σ → (τ → ν) ) :=
 by reflexivity
 
 lemma application_left_associative
 (σ τ ν : Type) (t : σ → τ → ν) (u : σ) (v : τ) :
-( t u v ) = ( (t u) v ) :=
+    ( t u v ) = ( (t u) v ) :=
 by reflexivity
 
 lemma lambda_right_associative
 (σ τ ν : Type) (t : ν) :
-( λx : σ, λy : τ, t ) = ( λx : σ, (λy : τ, t) ) :=
+    ( λx : σ, λy : τ, t ) = ( λx : σ, (λy : τ, t) ) :=
 by reflexivity
 
 lemma lambda_grouping
 (σ τ ν : Type) (t : ν) :
-( λ(x : σ)(y : τ), t ) = ( λx : σ, λy : τ, t ) :=
+    ( λ(x : σ)(y : τ), t ) = ( λx : σ, λy : τ, t ) :=
 by reflexivity
 
 lemma lambda_type_grouping
 (σ τ ν : Type) (t : ν) :
-( λ(x y : σ), t ) = ( λ(x : σ)(y : σ), t ) :=
+    ( λ(x y : σ), t ) = ( λ(x : σ)(y : σ), t ) :=
 by reflexivity
 
 constants a b : ℤ
@@ -57,6 +57,40 @@ inductive ArithmeticExpr : Type
 | sub : ArithmeticExpr → ArithmeticExpr → ArithmeticExpr
 | mul : ArithmeticExpr → ArithmeticExpr → ArithmeticExpr
 | div : ArithmeticExpr → ArithmeticExpr → ArithmeticExpr
+
+def eval (env : string → ℤ) : ArithmeticExpr → ℤ
+| (ArithmeticExpr.num i) := i
+| (ArithmeticExpr.sym s) := env s
+| (ArithmeticExpr.add e₁ e₂) := eval e₁ + eval e₂
+| (ArithmeticExpr.sub e₁ e₂) := eval e₁ - eval e₂
+| (ArithmeticExpr.mul e₁ e₂) := eval e₁ * eval e₂
+| (ArithmeticExpr.div e₁ e₂) := eval e₁ / eval e₂
+
+def example_env (key : string) : ℤ
+:= if key = "any" then 100 else string.to_nat key
+
+def example_eval : ℤ
+:= (eval example_env) (ArithmeticExpr.sub
+    (ArithmeticExpr.div
+        (ArithmeticExpr.add
+            (ArithmeticExpr.sym "any") (ArithmeticExpr.num 3)
+        )
+        (ArithmeticExpr.num 3)
+    )
+    (ArithmeticExpr.mul
+        (ArithmeticExpr.num 5) (ArithmeticExpr.sym "4")
+    )
+)
+def expected_eval : ℤ
+:= (100 + 3) / 3 - 5 * 4
+
+lemma fourteen :
+    example_eval = expected_eval ∧ example_eval = 14 :=
+begin
+apply and.intro,
+refl, -- example_eval = expected_eval
+refl -- example_eval = 14
+end
 
 inductive List (α : Type) : Type
 | nil : List
